Better Handling of Cache Invariants.

src/BinEncoders/Env/Common/ComposeOpt.v
@@ -4,9 +4,24 @@ Require Import
 
 Set Implicit Arguments.
 
-Lemma compose_encode_correct A A' B
-      (cache : Cache)
-      {P : CacheDecode -> Prop}
+Definition compose E B
+           (transformer : Transformer B)
+           (encode1 : E -> Comp (B * E))
+           (encode2 : E -> Comp (B * E)) :=
+  (fun e0 =>
+    `(p, e1) <- encode1 e0;
+    `(q, e2) <- encode2 e1;
+    ret (transform p q, e2))%comp.
+
+Notation "x 'Then' y" := (compose _ x y) (at level 100, right associativity).
+Notation "x 'Done'"   := (x Then fun e => ret (transform_id, e)) (at level 99, right associativity).
+
+Lemma compose_encode_correct
+      {A A' B}
+      {cache : Cache}
+      {P  : CacheDecode -> Prop}
+      {P_inv1 P_inv2 : (CacheDecode -> Prop) -> Prop}
+      (P_inv_pf : cache_inv_Property P (fun P => P_inv1 P /\ P_inv2 P))
       (transformer : Transformer B)
       (project : A -> A')
       (predicate : A -> Prop)
@@ -14,40 +29,43 @@ Lemma compose_encode_correct A A' B
       (encode1 : A' -> CacheEncode -> Comp (B * CacheEncode))
       (encode2 : A -> CacheEncode -> Comp (B * CacheEncode))
       (decode1 : B -> CacheDecode -> option (A' * B * CacheDecode))
-      (decode1_pf : encode_decode_correct_f cache transformer predicate' encode1 decode1 P)
-      (pred_pf : forall data, predicate data -> predicate' (project data))
+      (decode1_pf :
+         cache_inv_Property P P_inv1
+         -> encode_decode_correct_f cache transformer predicate' encode1 decode1 P)
       (decode2 : A' -> B -> CacheDecode -> option (A * B * CacheDecode))
       (decode2_pf : forall proj,
+          cache_inv_Property P P_inv2 ->
           encode_decode_correct_f cache transformer
             (fun data => predicate data /\ project data = proj)
             encode2
             (decode2 proj) P)
+      (pred_pf : forall data, predicate data -> predicate' (project data))
   : encode_decode_correct_f
       cache transformer predicate
       (fun (data : A) (ctx : CacheEncode) =>
-         `(bin, env') <- encode1 (project data) ctx;
-         `(bin', env'') <- encode2 data env';
-         ret (transform bin bin', env'')
+         compose _ (encode1 (project data)) (encode2 data)  ctx
       )%comp
      (fun (bin : B) (env : CacheDecode) =>
         `(proj, rest, env') <- decode1 bin env;
           decode2 proj rest env') P.
 Proof.
-  split.
+  unfold cache_inv_Property in *; split.
   { intros env env' xenv data bin ext env_pm pred_pm com_pf.
-    unfold Bind2 in com_pf; computes_to_inv; destruct v;
+    unfold compose, Bind2 in com_pf; computes_to_inv; destruct v;
       destruct v0.
-    destruct (proj1 decode1_pf _ _ _ _ _ (transform b0 ext) env_pm (pred_pf _ pred_pm) com_pf); intuition; simpl in *; injections.
-    setoid_rewrite <- transform_assoc; rewrite H0.
+    destruct (proj1 (decode1_pf (proj1 P_inv_pf)) _ _ _ _ _ (transform b0 ext) env_pm (pred_pf _ pred_pm) com_pf); intuition; simpl in *; injections.
+    setoid_rewrite <- transform_assoc; rewrite H2.
     simpl.
-    destruct (proj1 (decode2_pf (project data)) _ _ _ _ _ ext H1 (conj pred_pm (eq_refl _)) com_pf'); intuition; simpl in *; injections.
-    rewrite H2; eauto. }
+    destruct (proj1 (decode2_pf (project data) H1)
+                    _ _ _ _ _ ext H3 (conj pred_pm (eq_refl _)) com_pf');
+      intuition; simpl in *; injections.
+    eauto. }
   { intros.
     destruct (decode1 bin env') as [ [ [? ?] ? ] | ] eqn : ? ;
       simpl in *; try discriminate.
-    eapply (proj2 decode1_pf) in Heqo; eauto;
+    eapply (proj2 (decode1_pf (proj1 P_inv_pf))) in Heqo; eauto;
       destruct Heqo; destruct_ex; intuition;
-        eapply (proj2 (decode2_pf a)) in H1; eauto;
+        eapply (proj2 (decode2_pf a H5)) in H1; eauto;
           destruct H1; destruct_ex; intuition; subst.
     eexists; eexists; repeat split.
     repeat computes_to_econstructor; eauto.
