src/BinEncoders/Env/Lib2/EnumOpt.v
@@ -103,16 +103,16 @@ Section Enum.
   Qed.
 
   Theorem Enum_decode_correct
-    {P : CacheDecode -> Prop}
-      (P_OK : forall b cd, P cd -> P (addD cd b))
-    : NoDupVector tb
-    -> encode_decode_correct_f cache transformer (fun _ => True) encode_enum_Spec decode_enum P.
+          (tb_OK : NoDupVector tb)
+          {P : CacheDecode -> Prop}
+          (P_OK : cache_inv_Property P (fun P => forall b cd, P cd -> P (addD cd b)))
+    : encode_decode_correct_f cache transformer (fun _ => True) encode_enum_Spec decode_enum P.
   Proof.
     split; unfold encode_enum_Spec, decode_enum.
     { intros env env' xenv c c' ext Eeq Ppred Penc.
       destruct (proj1 (Word_decode_correct P_OK) _ _ _ _ _ ext Eeq I Penc) as [? [? ?] ].
-      rewrite H0; simpl.
-      apply (word_indexed_correct _ (ibound (indexb c))) in H.
+      rewrite H; simpl.
+      apply (word_indexed_correct _ (ibound (indexb c))) in tb_OK.
       subst; simpl in *.
       destruct (word_indexed (nth tb (ibound (indexb c))) tb);
         intros; simpl in *.
