src/BinEncoders/Env/Lib2/WordOpt.v
@@ -41,7 +41,7 @@ Section Word.
 
   Theorem Word_decode_correct
           {P : CacheDecode -> Prop}
-          (P_OK : forall b cd, P cd -> P (addD cd b))
+          (P_OK : cache_inv_Property P (fun P => forall b cd, P cd -> P (addD cd b)))
     :
     encode_decode_correct_f cache transformer (fun _ => True) encode_word_Spec decode_word P.
   Proof.
